Induct: converted some theories to new-style format;

src/HOL/Induct/Mutil.thy
@@ -1,29 +1,150 @@
-(*  Title:      HOL/Induct/Mutil
+(*  Title:      HOL/Induct/Mutil.thy
     ID:         $Id$
     Author:     Lawrence C Paulson, Cambridge University Computer Laboratory
     Copyright   1996  University of Cambridge
-
-The Mutilated Chess Board Problem, formalized inductively
-  Originator is Max Black, according to J A Robinson.
-  Popularized as the Mutilated Checkerboard Problem by J McCarthy
 *)
 
-Mutil = Main +
+header {* The Mutilated Chess Board Problem *}
 
-consts     tiling :: "'a set set => 'a set set"
+theory Mutil = Main:
+
+text {*
+  The Mutilated Chess Board Problem, formalized inductively.
+
+  Originator is Max Black, according to J A Robinson.  Popularized as
+  the Mutilated Checkerboard Problem by J McCarthy.
+*}
+
+consts tiling :: "'a set set => 'a set set"
 inductive "tiling A"
-  intrs
-    empty  "{} : tiling A"
-    Un     "[| a: A;  t: tiling A;  a Int t = {} |] ==> a Un t : tiling A"
+  intros [simp, intro]
+    empty: "{} \<in> tiling A"
+    Un: "a \<in> A ==> t \<in> tiling A ==> a \<inter> t = {} ==> a \<union> t \<in> tiling A"
 
-consts    domino :: "(nat*nat)set set"
+consts domino :: "(nat \<times> nat) set set"
 inductive domino
-  intrs
-    horiz  "{(i, j), (i, Suc j)} : domino"
-    vertl  "{(i, j), (Suc i, j)} : domino"
+  intros [simp]
+    horiz: "{(i, j), (i, Suc j)} \<in> domino"
+    vertl: "{(i, j), (Suc i, j)} \<in> domino"
 
 constdefs
-  coloured  :: "nat => (nat*nat)set"
-   "coloured b == {(i,j). (i+j) mod #2 = b}"
+  coloured :: "nat => (nat \<times> nat) set"
+   "coloured b == {(i, j). (i + j) mod #2 = b}"
+
+
+text {* \medskip The union of two disjoint tilings is a tiling *}
+
+lemma tiling_UnI [rule_format, intro]:
+  "t \<in> tiling A ==> u \<in> tiling A --> t \<inter> u = {} --> t \<union> u \<in> tiling A"
+  apply (erule tiling.induct)
+   prefer 2
+   apply (simp add: Un_assoc)
+  apply auto
+  done
+
+
+text {* \medskip Chess boards *}
+
+lemma Sigma_Suc1 [simp]:
+  "lessThan (Suc n) \<times> B = ({n} \<times> B) \<union> ((lessThan n) \<times> B)"
+  apply (unfold lessThan_def)
+  apply auto
+  done
+
+lemma Sigma_Suc2 [simp]:
+  "A \<times> lessThan (Suc n) = (A \<times> {n}) \<union> (A \<times> (lessThan n))"
+  apply (unfold lessThan_def)
+  apply auto
+  done
+
+lemma sing_Times_lemma: "({i} \<times> {n}) \<union> ({i} \<times> {m}) = {(i, m), (i, n)}"
+  apply auto
+  done
+
+lemma dominoes_tile_row [intro!]: "{i} \<times> lessThan (#2 * n) \<in> tiling domino"
+  apply (induct n)
+   apply (simp_all add: Un_assoc [symmetric])
+  apply (rule tiling.Un)
+    apply (auto simp add: sing_Times_lemma)
+  done
+
+lemma dominoes_tile_matrix: "(lessThan m) \<times> lessThan (#2 * n) \<in> tiling domino"
+  apply (induct m)
+   apply auto
+  done
+
+
+text {* \medskip @{term coloured} and Dominoes *}
+
+lemma coloured_insert [simp]:
+  "coloured b \<inter> (insert (i, j) t) =
+   (if (i + j) mod #2 = b then insert (i, j) (coloured b \<inter> t)
+    else coloured b \<inter> t)"
+  apply (unfold coloured_def)
+  apply auto
+  done
+
+lemma domino_singletons:
+  "d \<in> domino ==>
+    (\<exists>i j. coloured 0 \<inter> d = {(i, j)}) \<and>
+    (\<exists>m n. coloured 1 \<inter> d = {(m, n)})"
+  apply (erule domino.cases)
+   apply (auto simp add: mod_Suc)
+  done
+
+lemma domino_finite [simp]: "d \<in> domino ==> finite d"
+  apply (erule domino.cases)
+   apply auto
+  done
+
+
+text {* \medskip Tilings of dominoes *}
+
+lemma tiling_domino_finite [simp]: "t \<in> tiling domino ==> finite t"
+  apply (erule tiling.induct)
+   apply auto
+  done
+
+declare
+  Int_Un_distrib [simp]
+  Diff_Int_distrib [simp]
+
+lemma tiling_domino_0_1:
+  "t \<in> tiling domino ==> card (coloured 0 \<inter> t) = card (coloured 1 \<inter> t)"
+  apply (erule tiling.induct)
+   apply (drule_tac [2] domino_singletons)
+   apply auto
+  apply (subgoal_tac "\<forall>p C. C \<inter> a = {p} --> p \<notin> t")
+    -- {* this lemma tells us that both ``inserts'' are non-trivial *}
+   apply (simp (no_asm_simp))
+  apply blast
+  done
+
+
+text {* \medskip Final argument is surprisingly complex *}
+
+theorem gen_mutil_not_tiling:
+  "t \<in> tiling domino ==>
+    (i + j) mod #2 = 0 ==> (m + n) mod #2 = 0 ==>
+    {(i, j), (m, n)} \<subseteq> t
+  ==> (t - {(i, j)} - {(m, n)}) \<notin> tiling domino"
+  apply (rule notI)
+  apply (subgoal_tac
+    "card (coloured 0 \<inter> (t - {(i, j)} - {(m, n)})) <
+      card (coloured 1 \<inter> (t - {(i, j)} - {(m, n)}))")
+   apply (force simp only: tiling_domino_0_1)
+  apply (simp add: tiling_domino_0_1 [symmetric])
+  apply (simp add: coloured_def card_Diff2_less)
+  done
+
+text {* Apply the general theorem to the well-known case *}
+
+theorem mutil_not_tiling:
+  "t = lessThan (#2 * Suc m) \<times> lessThan (#2 * Suc n)
+    ==> t - {(0, 0)} - {(Suc (#2 * m), Suc (#2 * n))} \<notin> tiling domino"
+  apply (rule gen_mutil_not_tiling)
+     apply (blast intro!: dominoes_tile_matrix)
+    apply auto
+  done
 
 end
