src/HOL/Induct/ABexp.thy
@@ -2,52 +2,50 @@
     ID:         $Id$
     Author:     Stefan Berghofer, TU Muenchen
     Copyright   1998  TU Muenchen
-
-Arithmetic and boolean expressions
 *)
 
-ABexp = Main +
+header {* Arithmetic and boolean expressions *}
 
-datatype
-  'a aexp = IF ('a bexp) ('a aexp) ('a aexp)
-          | Sum ('a aexp) ('a aexp)
-          | Diff ('a aexp) ('a aexp)
-          | Var 'a
-          | Num nat
-and
-  'a bexp = Less ('a aexp) ('a aexp)
-          | And ('a bexp) ('a bexp)
-          | Neg ('a bexp)
+theory ABexp = Main:
+
+datatype 'a aexp =
+    IF "'a bexp"  "'a aexp"  "'a aexp"
+  | Sum "'a aexp"  "'a aexp"
+  | Diff "'a aexp"  "'a aexp"
+  | Var 'a
+  | Num nat
+and 'a bexp =
+    Less "'a aexp"  "'a aexp"
+  | And "'a bexp"  "'a bexp"
+  | Neg "'a bexp"
 
 
-(** evaluation of arithmetic and boolean expressions **)
+text {* \medskip Evaluation of arithmetic and boolean expressions *}
 
 consts
-  evala :: ('a => nat) => 'a aexp => nat
-  evalb :: ('a => nat) => 'a bexp => bool
+  evala :: "('a => nat) => 'a aexp => nat"
+  evalb :: "('a => nat) => 'a bexp => bool"
 
 primrec
-  "evala env (IF b a1 a2) =
-     (if evalb env b then evala env a1 else evala env a2)"
+  "evala env (IF b a1 a2) = (if evalb env b then evala env a1 else evala env a2)"
   "evala env (Sum a1 a2) = evala env a1 + evala env a2"
   "evala env (Diff a1 a2) = evala env a1 - evala env a2"
   "evala env (Var v) = env v"
   "evala env (Num n) = n"
 
   "evalb env (Less a1 a2) = (evala env a1 < evala env a2)"
-  "evalb env (And b1 b2) = (evalb env b1 & evalb env b2)"
-  "evalb env (Neg b) = (~ evalb env b)"
+  "evalb env (And b1 b2) = (evalb env b1 \<and> evalb env b2)"
+  "evalb env (Neg b) = (\<not> evalb env b)"
 
 
-(** substitution on arithmetic and boolean expressions **)
+text {* \medskip Substitution on arithmetic and boolean expressions *}
 
 consts
-  substa :: ('a => 'b aexp) => 'a aexp => 'b aexp
-  substb :: ('a => 'b aexp) => 'a bexp => 'b bexp
+  substa :: "('a => 'b aexp) => 'a aexp => 'b aexp"
+  substb :: "('a => 'b aexp) => 'a bexp => 'b bexp"
 
 primrec
-  "substa f (IF b a1 a2) =
-     IF (substb f b) (substa f a1) (substa f a2)"
+  "substa f (IF b a1 a2) = IF (substb f b) (substa f a1) (substa f a2)"
   "substa f (Sum a1 a2) = Sum (substa f a1) (substa f a2)"
   "substa f (Diff a1 a2) = Diff (substa f a1) (substa f a2)"
   "substa f (Var v) = f v"
@@ -56,5 +54,21 @@ primrec
   "substb f (Less a1 a2) = Less (substa f a1) (substa f a2)"
   "substb f (And b1 b2) = And (substb f b1) (substb f b2)"
   "substb f (Neg b) = Neg (substb f b)"
+
+lemma subst1_aexp_bexp:
+  "evala env (substa (Var (v := a')) a) = evala (env (v := evala env a')) a \<and>
+  evalb env (substb (Var (v := a')) b) = evalb (env (v := evala env a')) b"
+    --  {* one variable *}
+  apply (induct a and b)
+         apply simp_all
+  done
+
+lemma subst_all_aexp_bexp:
+  "evala env (substa s a) = evala (\<lambda>x. evala env (s x)) a \<and>
+  evalb env (substb s b) = evalb (\<lambda>x. evala env (s x)) b"
+    -- {* all variables *}
+  apply (induct a and b)
+         apply auto
+  done
 
 end
