src/HOL/Induct/Term.thy
@@ -2,23 +2,23 @@
     ID:         $Id$
     Author:     Stefan Berghofer,  TU Muenchen
     Copyright   1998  TU Muenchen
-
-Terms over a given alphabet -- function applications
 *)
 
-Term = Main +
+header {* Terms over a given alphabet *}
 
-datatype
-  ('a, 'b) term = Var 'a
-                | App 'b ((('a, 'b) term) list)
+theory Term = Main:
+
+datatype ('a, 'b) "term" =
+    Var 'a
+  | App 'b "('a, 'b) term list"
 
 
-(** substitution function on terms **)
+text {* \medskip Substitution function on terms *}
 
 consts
-  subst_term :: "['a => ('a, 'b) term, ('a, 'b) term] => ('a, 'b) term"
+  subst_term :: "('a => ('a, 'b) term) => ('a, 'b) term => ('a, 'b) term"
   subst_term_list ::
-    "['a => ('a, 'b) term, ('a, 'b) term list] => ('a, 'b) term list"
+    "('a => ('a, 'b) term) => ('a, 'b) term list => ('a, 'b) term list"
 
 primrec
   "subst_term f (Var a) = f a"
@@ -27,5 +27,36 @@ primrec
   "subst_term_list f [] = []"
   "subst_term_list f (t # ts) =
      subst_term f t # subst_term_list f ts"
+
+
+text {* \medskip A simple theorem about composition of substitutions *}
+
+lemma subst_comp:
+  "(subst_term ((subst_term f1) \<circ> f2) t) =
+    (subst_term f1 (subst_term f2 t)) \<and>
+  (subst_term_list ((subst_term f1) \<circ> f2) ts) =
+    (subst_term_list f1 (subst_term_list f2 ts))"
+  apply (induct t and ts rule: term.induct)
+     apply simp_all
+  done
+
+
+text {* \medskip Alternative induction rule *}
+
+lemma term_induct2:
+  "(!!v. P (Var v)) ==>
+    (!!f ts. list_all P ts ==> P (App f ts))
+  ==> P t"
+proof -
+  case antecedent
+  have "P t \<and> list_all P ts"
+    apply (induct t and ts rule: term.induct)
+       apply (rule antecedent)
+      apply (rule antecedent)
+      apply assumption
+     apply simp_all
+    done
+  thus ?thesis ..
+qed
 
 end
